rename variables for consistency

Instances/Monad.v
@@ -17,8 +17,8 @@ Implicit Type M : Type → Type.
 
 Section Identity_Monad.
   Definition bind_id {A B} 
-    (i : Identity A) (f : A → Identity B) : Identity B := 
-      match i with
+    (m : Identity A) (f : A → Identity B) : Identity B := 
+      match m with
       | identity a => f a
       end.
   
@@ -28,17 +28,17 @@ Section Identity_Monad.
     reflexivity.
   Qed.
 
-  Lemma bind_id_id_right : ∀ (A : Type) (ia : Identity A),
-    bind_id ia identity = ia.
+  Lemma bind_id_id_right : ∀ (A : Type) (m : Identity A),
+    bind_id m identity = m.
   Proof.
-    intros. destruct ia. reflexivity.
+    intros. destruct m. reflexivity.
   Qed.
 
-  Lemma bind_id_assoc : ∀ (A B C : Type) (ia : Identity A)
+  Lemma bind_id_assoc : ∀ (A B C : Type) (m : Identity A)
     (f : A → Identity B) (g : B → Identity C),
-    bind_id (bind_id ia f) g = bind_id ia (λ a : A, bind_id (f a) g).
+    bind_id (bind_id m f) g = bind_id m (λ a : A, bind_id (f a) g).
   Proof.
-    intros. destruct ia; simpl. reflexivity.
+    intros. destruct m; simpl. reflexivity.
   Qed.
 
   Lemma identity_inj : ∀ A (x y : A),
@@ -47,17 +47,8 @@ Section Identity_Monad.
     intros A x y H. inversion H. reflexivity.
   Qed.
 
-  Definition widen_id {A : Type} (i : Identity A) : Identity A := i.
-
-  Lemma widen_id_return : ∀ (A : Type) (a : A), widen_id (identity a) = identity a.
-  Proof.
-    intros. unfold widen_id. reflexivity.
-  Qed.
-
   Global Instance monad_identity : Monad Identity :=
   {
-    widen := @widen_id;
-    widen_return := widen_id_return;
     bind_id_left := bind_id_id_left;
     bind_id_right := bind_id_id_right;
     bind_assoc := bind_id_assoc;
@@ -66,10 +57,10 @@ End Identity_Monad.
 
 Section Maybe_Monad.
   Definition bind_maybe {A B} 
-    (m : Maybe A) (k : A -> Maybe B) : Maybe B :=
+    (m : Maybe A) (f : A -> Maybe B) : Maybe B :=
     match m with
     | None => None
-    | Just a => k a
+    | Just a => f a
     end.
   Arguments bind_maybe [A B].
   Hint Unfold bind_maybe : soundness.
@@ -79,35 +70,19 @@ Section Maybe_Monad.
   Proof. simple_solve. Qed.
   Arguments bind_maybe_id_left [A B] f a.
 
-  Lemma bind_maybe_id_right : ∀ {A} (MA : Maybe A), 
-    bind_maybe MA Just = MA.
+  Lemma bind_maybe_id_right : ∀ {A} (m : Maybe A), 
+    bind_maybe m Just = m.
   Proof. simple_solve. Qed.
   Arguments bind_maybe_id_right [A].
 
-  Lemma bind_maybe_assoc : ∀ {A B C} (MA : Maybe A) 
+  Lemma bind_maybe_assoc : ∀ {A B C} (m : Maybe A) 
     (f : A → Maybe B) (g : B → Maybe C),
-  bind_maybe (bind_maybe MA f) g = bind_maybe MA (λ a : A, bind_maybe (f a) g).
+  bind_maybe (bind_maybe m f) g = bind_maybe m (λ a : A, bind_maybe (f a) g).
   Proof. simple_solve. Qed.
-  Arguments bind_maybe_assoc [A B C] MA f g.
-
-  Lemma just_inj : ∀ A (x y : A),
-    Just x = Just y → x = y.
-  Proof. 
-    intros A x y Heq. inversion Heq. reflexivity.
-  Qed.
-
-  Definition widen_maybe {A : Type} (m : Maybe A) := (id (A:=Maybe A) m).
-
-  Lemma widen_maybe_return : ∀ (A : Type) (a : A),
-    widen_maybe (Just a) = Just a.
-  Proof.
-    unfold widen_maybe. intros. rewrite id_refl. reflexivity.
-  Qed.
+  Arguments bind_maybe_assoc [A B C] m f g.
 
   Global Instance monad_maybe : Monad Maybe :=
   {
-    widen := @widen_maybe;
-    widen_return := widen_maybe_return;
     bind_id_left := bind_maybe_id_left;
     bind_id_right := bind_maybe_id_right;
     bind_assoc := bind_maybe_assoc;
@@ -117,11 +92,11 @@ Hint Rewrite @bind_maybe_id_left @bind_maybe_id_right : soundness.
 
 Section AbstractMaybe_Monad.
   Definition bind_maybeA {A B : Type}
-    (m : AbstractMaybe A) (k : A -> AbstractMaybe B) : AbstractMaybe B :=
+    (m : AbstractMaybe A) (f : A -> AbstractMaybe B) : AbstractMaybe B :=
     match m with
     | NoneA => NoneA
-    | JustA a => k a
-    | JustOrNoneA a => match (k a) with
+    | JustA a => f a
+    | JustOrNoneA a => match (f a) with
                        | NoneA => NoneA
                        | JustA b => JustOrNoneA b
                        | JustOrNoneA b => JustOrNoneA b
@@ -135,36 +110,20 @@ Section AbstractMaybe_Monad.
   Proof. simple_solve. Qed.
   Arguments bind_maybeA_id_left [A B] f a.
 
-  Lemma bind_maybeA_id_right :  ∀ {A} (MA : AbstractMaybe A),
-    bind_maybeA MA JustA = MA.
+  Lemma bind_maybeA_id_right :  ∀ {A} (m : AbstractMaybe A),
+    bind_maybeA m JustA = m.
   Proof. solve_monad. Qed.
   Arguments bind_maybeA_id_right [A].
 
-  Lemma bind_maybeA_assoc : ∀ {A B C} (MA : AbstractMaybe A) 
+  Lemma bind_maybeA_assoc : ∀ {A B C} (m : AbstractMaybe A) 
     (f : A → AbstractMaybe B) (g : B → AbstractMaybe C),
-    bind_maybeA (bind_maybeA MA f) g =
-    bind_maybeA MA (λ a : A, bind_maybeA (f a) g).
+    bind_maybeA (bind_maybeA m f) g =
+    bind_maybeA m (λ a : A, bind_maybeA (f a) g).
   Proof. solve_monad. Qed.
-  Arguments bind_maybeA_assoc [A B C] MA f g.
-
-  Lemma justA_inj : ∀ A (x y : A),
-    JustA x = JustA y → x = y.
-  Proof.
-    intros A x y Heq. inversion Heq. reflexivity.
-  Qed.
-
-  Definition widen_maybeA {A : Type} (am : AbstractMaybe A) := id am.
-
-  Lemma widen_maybeA_return : ∀ A (a : A),
-    widen_maybeA (JustA a) = JustA a.
-  Proof.
-    intros. unfold widen_maybeA. rewrite id_refl. reflexivity.
-  Qed.
+  Arguments bind_maybeA_assoc [A B C] m f g.
 
   Global Instance monad_abstract_maybe : Monad AbstractMaybe :=
   {
-    bindM := bind_maybeA;
-    widen_return := widen_maybeA_return;
     bind_id_left := bind_maybeA_id_left;
     bind_id_right := bind_maybeA_id_right;
     bind_assoc := bind_maybeA_assoc;
@@ -175,15 +134,15 @@ Hint Rewrite @bind_maybeA_id_left @bind_maybeA_id_right : soundness.
 Section MaybeT_Monad.
   Context {M} `{M_monad : Monad M}.
 
-  Definition bind_maybeT {A B} (x : MaybeT M A) 
+  Definition bind_maybeT {A B} (m : MaybeT M A) 
     (f : A -> MaybeT M B) : MaybeT M B :=
-    bindM (M:=M) x (λ v : Maybe A,
+    bindM (M:=M) m (λ v : Maybe A,
       match v with
       | None => NoneT
       | Just a => f a
       end
     ).
-  Arguments bind_maybeT [A B] x f.
+  Arguments bind_maybeT [A B] m f.
   Hint Unfold bind_maybeT : soundness.
 
   Lemma bind_maybeT_id_left : ∀ {A B} (f : A → MaybeT M B) (a : A), 
@@ -194,40 +153,28 @@ Section MaybeT_Monad.
   Qed.
   Arguments bind_maybeT_id_left [A B] f a.
 
-  Lemma bind_maybeT_id_right : ∀ {A} (MA : MaybeT M A),
-    bind_maybeT MA JustT = MA.
+  Lemma bind_maybeT_id_right : ∀ {A} (m : MaybeT M A),
+    bind_maybeT m JustT = m.
   Proof. 
     intros. unfold bind_maybeT, NoneT, JustT. 
-    replace (MA) with (bindM (M:=M) MA returnM) at 2.
-    f_equal. ext; destruct x; reflexivity.
-    rewrite <- (bind_id_right (M:=M)). reflexivity.
+    rewrite <- (bind_id_right (M:=M)). f_equal. 
+    ext; destruct x; reflexivity.
   Qed.
-  Arguments bind_maybeT_id_right [A] MA.
+  Arguments bind_maybeT_id_right [A] m.
 
-  Lemma bind_maybeT_assoc : ∀ {A B C} (MA : MaybeT M A) 
+  Lemma bind_maybeT_assoc : ∀ {A B C} (m : MaybeT M A) 
     (f : A → MaybeT M B) (g : B → MaybeT M C),
-    bind_maybeT (bind_maybeT MA f) g =
-    bind_maybeT MA (λ a : A, bind_maybeT (f a) g).
+    bind_maybeT (bind_maybeT m f) g =
+    bind_maybeT m (λ a : A, bind_maybeT (f a) g).
   Proof. 
     intros. unfold bind_maybeT. autorewrite with soundness.
     f_equal. ext. destruct x; eauto with soundness.
     unfold NoneT. autorewrite with soundness. reflexivity.
   Qed.
-  Arguments bind_maybeT_assoc [A B C] MA f g.
-
-  Definition widen_maybeT {A : Type} (m : MaybeT M A) : MaybeT M A := 
-    (id (widen (M:=M) m)).
-
-  Lemma widen_maybeT_return : ∀ A (a : A),
-    widen_maybeT (returnM (M:=M) (Just a)) = returnM (M:=M) (Just a).
-  Proof.
-    intros. unfold widen_maybeT. rewrite id_refl. rewrite widen_return.
-    reflexivity.
-  Qed.
+  Arguments bind_maybeT_assoc [A B C] m f g.
 
   Global Instance monad_maybeT : Monad (MaybeT M) :=
   {
-    widen_return := widen_maybeT_return;
     bind_id_left := bind_maybeT_id_left;
     bind_id_right := bind_maybeT_id_right;
     bind_assoc := bind_maybeT_assoc;
@@ -239,17 +186,17 @@ Hint Rewrite @bind_maybeT_id_left @bind_maybeT_id_right : soundness.
 Section MaybeT_MonadT.
   Context {M} `{M_monad : Monad M}.
   
-  Definition lift_maybeT {A} (Ma : M A) : MaybeT M A :=
-    bindM (M:=M) Ma (λ a, JustT a).
+  Definition lift_maybeT {A} (m : M A) : MaybeT M A :=
+    bindM (M:=M) m (λ a, JustT a).
   Arguments lift_maybeT [_] _.
   Hint Unfold lift_maybeT : soundness.
 
-  Lemma lift_maybeT_pure : ∀ (A : Type) (x : A),
-    lift_maybeT (returnM x) = returnM x.
+  Lemma lift_maybeT_pure : ∀ (A : Type) (a : A),
+    lift_maybeT (returnM a) = returnM a.
   Proof. solve_monad. Qed.
 
-  Lemma lift_maybeT_bind : ∀ (A B : Type) (x : M A) (f : A → M B),
-  lift_maybeT (x >>= f) = bind_maybeT (lift_maybeT x) (f ∘ (lift_maybeT (A:=B))).
+  Lemma lift_maybeT_bind : ∀ (A B : Type) (m : M A) (f : A → M B),
+  lift_maybeT (m >>= f) = bind_maybeT (lift_maybeT m) (f ∘ (lift_maybeT (A:=B))).
   Proof. 
     intros. unfold lift_maybeT, bind_maybeT, NoneT, JustT. 
     autorewrite with soundness. f_equal; ext. autorewrite with soundness.
@@ -264,7 +211,7 @@ Section MaybeT_MonadT.
 End MaybeT_MonadT.
 
 Section MaybeAT_Monad.
-  Context {M} `{M_monad : Monad M} `{JoinableMonad M}.
+  Context {M} `{M_monad : Monad M}.
 
   Definition bind_maybeAT {A B} 
     (Mma : MaybeAT M A)
@@ -291,18 +238,18 @@ Section MaybeAT_Monad.
   Qed.
   Arguments bind_maybeAT_id_left [A B] f a.
 
-  Lemma bind_maybeAT_id_right : ∀ (A : Type) (MA : MaybeAT M A), 
-    bind_maybeAT MA JustAT = MA.
+  Lemma bind_maybeAT_id_right : ∀ (A : Type) (m : MaybeAT M A), 
+    bind_maybeAT m JustAT = m.
   Proof. 
     unfold bind_maybeAT, JustAT. intros. rewrite <- (bind_id_right (M:=M)).
     f_equal; extensionality x. 
     destruct x; autorewrite with soundness; try reflexivity.
   Qed.
 
-  Lemma bind_maybeAT_assoc : ∀ {A B C} (MA : MaybeAT M A) 
+  Lemma bind_maybeAT_assoc : ∀ {A B C} (m : MaybeAT M A) 
     (f : A → MaybeAT M B) (g : B → MaybeAT M C),
-    bind_maybeAT (bind_maybeAT MA f) g =
-    bind_maybeAT MA (λ a : A, bind_maybeAT (f a) g).
+    bind_maybeAT (bind_maybeAT m f) g =
+    bind_maybeAT m (λ a : A, bind_maybeAT (f a) g).
   Proof. 
     intros. unfold bind_maybeAT. autorewrite with soundness.
     f_equal; ext. destruct x; simpl. reflexivity. autorewrite with soundness.
@@ -313,21 +260,11 @@ Section MaybeAT_Monad.
     autorewrite with soundness. reflexivity.
     autorewrite with soundness. reflexivity.
   Qed.
-  Arguments bind_maybeAT_assoc [A B C] MA f g.
-
-  Definition widen_maybeAT {A : Type} (m : MaybeAT M A) : MaybeAT M A := 
-    (id (widen (M:=M) m)).
-
-  Lemma widen_maybeAT_return : ∀ A (a : A),
-    widen_maybeAT (returnM (M:=M) (JustA a)) = returnM (M:=M) (JustA a).
-  Proof.
-    intros. unfold widen_maybeAT. rewrite id_refl, widen_return. reflexivity.
-  Qed.
+  Arguments bind_maybeAT_assoc [A B C] m f g.
 
   Global Instance monad_maybeAT 
   : Monad (MaybeAT M) :=
   {
-    widen_return := widen_maybeAT_return;
     bind_id_left := bind_maybeAT_id_left;
     bind_id_right := bind_maybeAT_id_right;
     bind_assoc := bind_maybeAT_assoc;
@@ -338,26 +275,26 @@ Hint Unfold bind_maybeAT : soundness.
 Section MaybeAT_MonadT.
   Context {M} `{M_monad : Monad M}.
 
-  Definition lift_maybeAT {A} (Ma : M A) : MaybeAT M A :=
-    bindM (M:=M) Ma (λ a, JustAT a).
+  Definition lift_maybeAT {A} (m : M A) : MaybeAT M A :=
+    bindM (M:=M) m (λ a, JustAT a).
   Arguments lift_maybeAT [A].
   Hint Unfold lift_maybeAT : soundness.
 
-  Definition lift_maybeAT_pure : ∀ {A} (x : A),
-    lift_maybeAT (returnM x) = returnM x.
+  Definition lift_maybeAT_pure : ∀ {A} (a : A),
+    lift_maybeAT (returnM a) = returnM a.
   Proof.
     solve_monad.
   Qed.
-  Arguments lift_maybeAT_pure [A] x.
+  Arguments lift_maybeAT_pure [A] a.
 
-  Definition lift_maybeAT_bind : ∀ {A B} (x : M A) (f : A → M B),
-    lift_maybeAT (x >>= f) = bind_maybeAT (lift_maybeAT x) (f ∘ lift_maybeAT (A:=B)).
+  Definition lift_maybeAT_bind : ∀ {A B} (m : M A) (f : A → M B),
+    lift_maybeAT (m >>= f) = bind_maybeAT (lift_maybeAT m) (f ∘ lift_maybeAT (A:=B)).
   Proof. 
     unfold lift_maybeAT, bind_maybeAT, JustAT. intros.
     autorewrite with soundness. f_equal; ext. autorewrite with soundness.
     reflexivity.
   Qed.
-  Arguments lift_maybeAT_bind [A B] x f.
+  Arguments lift_maybeAT_bind [A B] m f.
 
   Global Instance monadT_maybeAT : MonadT MaybeAT :=
   {
@@ -372,47 +309,29 @@ Section State_Monad.
   Definition return_state {A} (a :A) : State S A := 
     λ st : S, (a, st).
 
-  Lemma return_state_inj : ∀ A (x y : A),
-    return_state x = return_state y → x = y.
-  Proof.
-    intros A x y H. unfold return_state in H. unfold Inhabited in S_inhabited.
-    eapply equal_f in H. Unshelve. inversion H. reflexivity. apply S_inhabited.
-  Qed.
-
   Definition bind_state {A B} 
-    (p : State S A) (k : A -> State S B) : State S B :=
-    λ st, let (x, st') := (p st) in k x st'.
+    (m : State S A) (f : A -> State S B) : State S B :=
+    λ st, let (x, st') := (m st) in f x st'.
 
-  Arguments bind_state [A B] p k.
+  Arguments bind_state [A B] m f.
   Hint Unfold bind_state : soundness.
 
   Lemma bind_state_id_left : ∀ (A B : Type) (f : A → State S B) (a : A),
     bind_state (return_state a) f = f a.
   Proof. simple_solve. Qed.
 
-  Lemma bind_state_id_right : ∀ (A : Type) (MA : State S A),
-    bind_state MA return_state = MA.
+  Lemma bind_state_id_right : ∀ (A : Type) (m : State S A),
+    bind_state m return_state = m.
   Proof. simple_solve. Qed.
 
-  Lemma bind_state_assoc : ∀ (A B C : Type) (MA : State S A) 
+  Lemma bind_state_assoc : ∀ (A B C : Type) (m : State S A) 
     (f : A → State S B) (g : B → State S C),
-    bind_state (bind_state MA f) g =
-    bind_state MA (λ a : A, bind_state (f a) g).
+    bind_state (bind_state m f) g =
+    bind_state m (λ a : A, bind_state (f a) g).
   Proof. simple_solve. Qed.
 
-  Definition widen_state {A : Type} (s : State S A) :=
-    λ st, let (a, st') := (s st) in (a, st ⊔ st').
-
-  Lemma widen_state_return : ∀ A (a : A),
-    widen_state (return_state a) = return_state a.
-  Proof.
-    unfold return_state, widen_state. intros. ext. rewrite join_idem.
-    reflexivity.
-  Qed.
-  
   Global Instance monad_state : Monad (State S) :=
   {
-    widen_return := widen_state_return;
     bind_id_left := bind_state_id_left;
     bind_id_right := bind_state_id_right;
     bind_assoc := bind_state_assoc;
@@ -422,17 +341,16 @@ Hint Unfold bind_state : soundness.
 
 Section Monad_StateT.
   Context {M} `{M_monad : Monad M}.
-  Context {S : Type} `{S_inhabited : !Inhabited S} `{S_joinable : Joinable S}.
+  Context {S : Type} `{S_inhabited : !Inhabited S}.
 
   Definition return_stateT {A} (a : A) :=
     λ st : S, returnM (a, st).
   Hint Unfold return_stateT : soundness.
 
-  Definition bind_stateT {A B} (MA : StateT S M A) 
+  Definition bind_stateT {A B} (m : StateT S M A) 
     (f : A -> StateT S M B) : StateT S M B :=
-    fun st => bindM (MA st) 
-      (fun p : (A*S)%type => let (a,st') := p in f a st').
-  Arguments bind_stateT [A B] MA f.
+    λ st, m st >>= λ p : (A*S)%type, let (a,st') := p in f a st'.
+  Arguments bind_stateT [A B] m f.
   Hint Unfold bind_stateT : soundness.
 
   Lemma bind_stateT_id_left : ∀ (A B : Type) (f : A → StateT S M B) (a : A), 
@@ -443,39 +361,28 @@ Section Monad_StateT.
   Qed.
   Arguments bind_stateT_id_left [A B] f a.
 
-  Lemma bind_stateT_id_right : ∀ (A : Type) (MA : StateT S M A), 
-    bind_stateT MA return_stateT = MA.
+  Lemma bind_stateT_id_right : ∀ (A : Type) (m : StateT S M A), 
+    bind_stateT m return_stateT = m.
   Proof.
     intros. autounfold with soundness. ext.
     rewrite <- bind_id_right. f_equal. ext. destruct x0.
     reflexivity.
   Qed.
-  Arguments bind_stateT_id_right [A] MA.
+  Arguments bind_stateT_id_right [A] m.
 
-  Lemma bind_stateT_assoc : ∀ (A B C : Type) (MA : StateT S M A) 
+  Lemma bind_stateT_assoc : ∀ (A B C : Type) (m : StateT S M A) 
     (f : A → StateT S M B) (g : B → StateT S M C),
-    bind_stateT (bind_stateT MA f) g =
-    bind_stateT MA (λ a : A, bind_stateT (f a) g).
+    bind_stateT (bind_stateT m f) g =
+    bind_stateT m (λ a : A, bind_stateT (f a) g).
   Proof.
     intros. autounfold with soundness. ext.
-    autorewrite with soundness. f_equal. ext.
-    destruct x0. reflexivity.
+    autorewrite with soundness. f_equal. extensionality p.
+    destruct p. reflexivity.
   Qed.
-  Arguments bind_stateT_assoc [A B C] MA f g.
+  Arguments bind_stateT_assoc [A B C] m f g.
 
-  Definition widen_stateT {A : Type} (s : StateT S M A) :=
-    λ st, let m := (s st) in widen m.
-
-  Lemma widen_stateT_return : ∀ A (a : A),
-    widen_stateT (return_stateT a) = return_stateT a.
-  Proof.
-    intros. unfold widen_stateT, return_stateT. ext. rewrite widen_return.
-    reflexivity.
-  Qed.
-  
   Global Instance monad_stateT : Monad (StateT S M) :=
   {
-    widen_return := widen_stateT_return;
     bind_id_left := bind_stateT_id_left;
     bind_id_right := bind_stateT_id_right;
     bind_assoc := bind_stateT_assoc;
@@ -487,27 +394,27 @@ Section MonadT_StateT.
   Context {M} `{M_monad :Monad M}.
   Context {S : Type} `{!Inhabited S}.
 
-  Definition lift_stateT {A} (MA : M A) : StateT S M A :=
-    fun st => bindM MA (fun a => returnM (a, st)).
-  Arguments lift_stateT [A] MA.
+  Definition lift_stateT {A} (m : M A) : StateT S M A :=
+    λ st, m >>= λ a, returnM (a, st).
+  Arguments lift_stateT [A] m.
   Hint Unfold lift_stateT : soundness.
   
-  Lemma lift_stateT_pure : ∀ (A : Type) (x : A), 
-    lift_stateT (returnM x) = return_stateT x.
+  Lemma lift_stateT_pure : ∀ (A : Type) (m : A), 
+    lift_stateT (returnM m) = return_stateT m.
   Proof.
     intros. autounfold with soundness. ext.
     autorewrite with soundness. reflexivity.
   Qed.
-  Arguments lift_stateT_pure [A] x.
+  Arguments lift_stateT_pure [A] m.
 
-  Lemma lift_stateT_bind : ∀ (A B : Type) (x : M A) (f : A → M B),
-    lift_stateT (x >>= f) = bind_stateT (lift_stateT x) (f ∘ lift_stateT (A:=B)).
+  Lemma lift_stateT_bind : ∀ (A B : Type) (m : M A) (f : A → M B),
+    lift_stateT (m >>= f) = bind_stateT (lift_stateT m) (f ∘ lift_stateT (A:=B)).
   Proof.
     intros. simpl.
     autounfold with soundness. ext. autorewrite with soundness.
     f_equal. ext. autorewrite with soundness. reflexivity.
   Qed.
-  Arguments lift_stateT_bind [A B] x f.
+  Arguments lift_stateT_bind [A B] m f.
 
   Global Instance monadT_stateT : MonadT (StateT S) :=
   {
